Es gilt zu zeigen, dass gilt: \\
$\lnot ( \lnot A \land \lnot C ) \lor ( A \land (\lnot B \lor A)) \equiv A \lor C$\\

Für $\lnot ( \lnot A \land \lnot C ) \lor ( A \land (\lnot B \lor A)) $:\\
\begin{center}
\begin{tabular}[h]{c|c|c|c}
 $A$ & $B$ & $C$ &  $\lnot ( \lnot A \land \lnot C ) \lor ( A \land (\lnot B \lor A))$ \\ 
 \hline
 1 & 1 & 1 & (~~1~~~0~~~0~~~0~~~*1~~~1~~0~~~1~~)\\
 1 & 1 & 0 & (~~1~~~0~~~0~~~1~~~*1~~~1~~~0~~~1~~)\\
 1 & 0 & 1 & (~~1~~~0~~~0~~~0~~~*1~~~1~~~1~~~1~~)\\
 1 & 0 & 0 & (~~1~~~0~~~0~~~1~~~*1~~~1~~~1~~~1~~)\\
 0 & 1 & 1 & (~~1~~~1~~~0~~~0~~~*1~~~0~~~0~~~0~~)\\
 0 & 1 & 0 & (~~0~~~1~~~1~~~1~~~*0~~~0~~~0~~~0~~)\\
 0 & 0 & 1 & (~~1~~~1~~~0~~~0~~~*1~~~0~~~1~~~1~~)\\
 0 & 0 & 0 & (~~0~~~1~~~1~~~1~~~*0~~~0~~~1~~~1~~)\\

\end{tabular}
\end{center}
\vspace{2cm}

Für $A \lor C$
\begin{center}
	\begin{tabular}[h]{c|c|c|c}
		$A$ & $B$ &  $C$ & $A \lor C$ \\ 
		\hline
		1 & 1 & 1 & 1\\
		1 & 1 & 0 & 1\\
		1 & 0 & 1 & 1\\
		1 & 0 & 0 & 1\\
		0 & 1 & 1 & 1\\
		0 & 1 & 0 & 0\\
		0 & 0 & 1 & 1\\
		0 & 0 & 0 & 0\\
	\end{tabular}
\end{center}

\vspace{1cm}
$ \left(1,1,1,1,1,1,0,1,0\right) \equiv \left(1,1,1,1,1,1,0,1,0\right) $\\
Die Aussagen sind äquivalent.